```haskell
{-
///////////////////////////////////////////////////////////////////////////////////////////////
<Ch.5-Ex.9> Show how a list comprehension can be used to define a function
scalarproduct :: [Int] -> [Int] -> Int that returns the scalar product of two lists. For
example:
> scalarproduct [1,2,3] [4,5,6]
32
///////////////////////////////////////////////////////////////////////////////////////////////
-}

-- manually summing elements
mysum :: [Int] -> Int
mysum [] = 0
mysum (x:xs) = x + mysum(xs)

--scalar product using zip
scalarproduct :: [Int] -> [Int] -> Int
scalarproduct xs ys = mysum [ x * y | (x, y) <- zip xs ys]

-- main
main = do
       putStr "[1, 2, 3] . [4, 5, 6] = "
       print (scalarproduct [1, 2, 3] [4, 5, 6])
       putStr "[1, 1, 1] . [2, 2, 2] = "
       print (scalarproduct [1, 1, 1] [2, 2, 2])
       putStr "[5, 6, 7] . [10, 8, 9] = "
       print (scalarproduct [5, 6, 7] [10, 8, 9])
```

Running the program grom ghci:
```cmd
*Main> :main
[1, 2, 3] . [4, 5, 6] = 32
[1, 1, 1] . [2, 2, 2] = 6
[5, 6, 7] . [10, 8, 9] = 161
```

The scalarproduct function determines a list by zipping 2 lists together and then multiplying
the components. Finally mysum recursively sums up all the results from our previously determined list.
